resolve one problem with adam's proof (S blocks and skip instead of irr_l resulted in putting an oracle *output* on the right list). possibly a similar problem in the loop proof? skipping the oracle's *output* is not going to match up with the inputs? or maybe i should use outputs-as-inputs strategy? what did he do that succeeded in PRF_DRBG?

src/examples/HMAC_DRBG_nonadaptive_LB.v
@@ -1,16 +1,18 @@
 Set Implicit Arguments.
 
-Require Import FCF.
+Require Import fcf.FCF.
 (* RndInList has a useful theorem (qam_count) about counting calls to an oracle. *)
-Require Import RndInList.
-Require Import HasDups.
-Require Import CompFold.
-Require Import PRF.
-Require Import OracleHybrid.
+Require Import fcf.RndInList.
+Require Import fcf.HasDups.
+Require Import fcf.CompFold.
+Require Import fcf.PRF.
+Require Import fcf.OracleHybrid.
 Require Import List.
-Require Import PRF_DRBG.        (* note: had to move PRF_DRBG into FCF dir for this *)
+Require Import fcf.PRF_DRBG.        (* note: had to move PRF_DRBG into FCF dir for this *)
 Require Import Coq.Program.Wf.
-Require Import OracleCompFold.
+Require Import fcf.OracleCompFold.
+
+Require Import fcf.Tactics.
 
 (* Shortcuts for FCF tactics *)
 (* TODO remove / inline these *)
@@ -86,15 +88,21 @@ Qed.
 Local Open Scope list_scope.
 Local Opaque evalDist.
 
+(* Spec says "V || 0x00"; here we will use a list of 8 bits of 0 (a byte) *)
+Fixpoint replicate {A} (n : nat) (a : A) : list A :=
+  match n with
+  | O => nil
+  | S n' => a :: replicate n' a
+  end.
+
+
 (* --- Begin my HMAC-DRBG spec --- *)
 Section PRG.
 
   (* note: the domain of the f is now Blist, not an abstract D
 the key type is now also Bvector eta, since HMAC specifies that the key has the same size as the output (simplified) *)
-(* Variable eta : nat. *)
-Definition eta:=1%nat.
-Opaque eta.
-(* coq gets stuck on an fcf_skip around line 256 *)
+Variable eta : nat.
+(* Definition eta:=256%nat. *) (* coq gets stuck on an fcf_skip around line 256 *)
 
 (* Variable RndK : Comp (Bvector eta). *)
 (* Variable RndV : Comp (Bvector eta). *)
@@ -108,8 +116,7 @@ Variable f : Bvector eta -> Blist -> Bvector eta.
 
 Definition KV : Set := (Bvector eta * Bvector eta)%type.
 Hypothesis eqDecState : EqDec KV.
-(* Variable eqdbv : EqDec (Bvector eta). *)
-Definition eqdbv := Bvector_EqDec eta.
+Variable eqdbv : EqDec (Bvector eta).
 Variable eqdbl : EqDec Blist.
 
 (* injection is to_list. TODO prove this *)
@@ -163,11 +170,11 @@ output: list (Bvector eta)
 state: k, v *)
 
 (* Spec says "V || 0x00"; here we will use a list of 8 bits of 0 (a byte) *)
-Fixpoint replicate {A} (n : nat) (a : A) : list A :=
+(*Fixpoint replicate {A} (n : nat) (a : A) : list A :=
   match n with
   | O => nil
   | S n' => a :: replicate n' a
-  end.
+  end.*)
 
 Definition zeroes : list bool := replicate 8 true.
 
@@ -255,6 +262,54 @@ Definition GenUpdate_rb (n : nat) : Comp (list (Bvector eta)) :=
 
 (* TODO: prove well_formed for the oracles *)
 
+
+(* oracleMap hardcodes acc for compFold as nil, so generalize it *)
+(*LENB: moved HERE to REMOVE DEPENDENCE ON Hypothesis H_numCalls : numCalls > 0*)
+Theorem compFold_acc blocksPerCall: forall numCalls bits acc state,
+   comp_spec
+     (fun x y : list (list (Bvector eta)) * KV =>
+      hd_error (fst x) = Some bits /\ tl (fst x) = fst y)
+     (compFold (pair_EqDec (list_EqDec (list_EqDec eqdbv)) eqDecState)
+        (fun (acc : list (list (Bvector eta)) * KV) (d : nat) =>
+         [rs, s]<-2 acc;
+         z <-$ GenUpdate_original s d; [r, s0]<-2 z; ret (rs ++ r :: nil, s0))
+        (bits :: acc, state) (replicate numCalls blocksPerCall))
+     (compFold (pair_EqDec (list_EqDec (list_EqDec eqdbv)) eqDecState)
+        (fun (acc : list (list (Bvector eta)) * KV) (d : nat) =>
+         [rs, s]<-2 acc;
+         z <-$ GenUpdate_original s d; [r, s0]<-2 z; ret (rs ++ r :: nil, s0))
+        (acc, state) (replicate numCalls blocksPerCall)).
+Proof. 
+  induction numCalls; intros.
+  - simpl. fcf_spec_ret.
+  - simpl.
+    fcf_inline_first. fcf_skip.
+    remember a0 as bits1. remember b as state'. clear Heqbits1 Heqstate'.
+    fcf_simp.
+    apply IHnumCalls. 
+Qed.
+Theorem comp_spec_acc_2  blocksPerCall: forall numCalls acc k v,
+ comp_spec (fun x y : list (list (Bvector eta)) * KV => fst x = fst y)
+     (compFold (pair_EqDec (list_EqDec (list_EqDec eqdbv)) eqDecState)
+        (fun (acc : list (list (Bvector eta)) * KV) (d : nat) =>
+         [rs, s]<-2 acc;
+         z <-$ GenUpdate_original s d; [r, s0]<-2 z; ret (rs ++ r :: nil, s0))
+        (acc,
+        (k, f k (to_list v)))
+        (replicate numCalls blocksPerCall))
+     (compFold (pair_EqDec (list_EqDec (list_EqDec eqdbv)) eqDecState)
+        (fun (acc : list (list (Bvector eta)) * KV) (d : nat) =>
+         [rs, s]<-2 acc;
+         z <-$ GenUpdate s d; [r, s0]<-2 z; ret (rs ++ r :: nil, s0))
+        (acc, (k, v))
+        (replicate numCalls blocksPerCall)).
+Proof.
+  induction numCalls; intros.
+  * simpl. fcf_spec_ret.
+  * simpl.
+    fcf_inline_first. fcf_simp. apply IHnumCalls.
+Qed.
+
 (* Non-adaptive adversary. Consequently, does not use OracleComp, because it won't be adjusting its input to the GenUpdate oracle (number of blocks requested from Gen_loop) based on the GenUpdate oracle's output, because the number of blocks and queries is fixed. *)
 Variable A : list (list (Bvector eta)) -> Comp bool.
 Hypothesis A_wf : forall ls, well_formed_comp (A ls).
@@ -316,7 +371,8 @@ Definition G1_prg_original_split : Comp bool :=
 
 (* use version that's better for induction *)
 
-(* oracleMap hardcodes acc for compFold as nil, so generalize it *)
+(* oracleMap hardcodes acc for compFold as nil, so generalize it 
+LENB: MOVE UP, AND SIMPLIFIED PROOF
 Theorem compFold_acc : forall numCalls bits acc state,
    comp_spec
      (fun x y : list (list (Bvector eta)) * KV =>
@@ -343,7 +399,7 @@ Proof.
     remember a0 as bits1. remember b as state'. clear Heqbits1 Heqstate'.
     fcf_simp.
     apply IHnumCalls0.
-Qed.
+Qed. *)
 
 (* do first call of map separately *)
 Theorem GenUpdate_split_close :
@@ -369,12 +425,13 @@ Proof.
 
     fcf_skip.
     instantiate (1 := (fun x y => hd_error (fst x) = Some bits /\ tail (fst x) = fst y)).
-    - apply compFold_acc.
+    - apply compFold_acc. 
     - fcf_simp. simpl in H5. inversion H5. clear H5. destruct a1. inversion H6. simpl in *. inversion H6. subst. fcf_reflexivity.
       Transparent GenUpdate_original.
 Qed.
 
 (* generalize acc again. could be generalized further for the function on v but oh well *)
+(*LENB: MOVED UP
 Theorem comp_spec_acc_2 : forall numCalls acc k v,
  comp_spec (fun x y : list (list (Bvector eta)) * KV => fst x = fst y)
      (compFold (pair_EqDec (list_EqDec (list_EqDec eqdbv)) eqDecState)
@@ -397,7 +454,7 @@ Proof.
   * simpl. fcf_spec_ret.
   * simpl.
     fcf_inline_first. fcf_simp. apply IHnumCalls'.
-Qed.
+Qed.*)
 
 (* G1_prg_original: calls GenUpdate_original, then GenUpdate_original
 G1_prg: uses GenUpdate_noV, then GenUpdate (v moved) *)
@@ -425,6 +482,8 @@ Proof.
     unfold oracleMap.
 
     - apply comp_spec_acc_2.
+(*LENB: if I don't move the definition of comp_spec_acc_2 up, I get 
+  "Error: comp_spec_acc_2 depends on the variable H_numCalls which is not declared in the context." here*)
 
     - fcf_simp. simpl in *. subst. fcf_reflexivity.
 Qed.
@@ -1063,7 +1122,7 @@ Solve All Obligations.          (* maybe the obligations are different? *)
 Next Obligation.
   clear segment; simpl.
   rename wildcard' into a. rename wildcard'0 into l. rename wildcard'1 into n.
-  specialize (skipn_length' n l). intros.
+  (*specialize (skipn_length' n l). intros.*)
   (* omega. *)
 Admitted.
 Close Scope nat.
@@ -1353,63 +1412,6 @@ PRF_Advantage_Game i = PRF_Advantage (the normal one with just the PRF/RF differ
     fcf_to_prhl_eq.
     admit.
 Qed.
-
-
-(* Below can be used to establish a maximum advantage over all constructed adversaries *)
-Theorem gtRat_impl_leRat:
-  forall a b,
-    (a <= b -> False) ->
-    b <= a.
-
-    intuition.
-    rattac.
-    destruct (le_dec (n * x) (n0 * x0))%nat.
-    trivial.
-    exfalso.
-    eapply H.
-    rattac.
-Qed.
-
-Fixpoint argMax(f : nat -> Rat) (n : nat) :=
-  match n with
-    | O => O
-    | S n' => let p := (argMax f n') in
-              if (le_Rat_dec (f (S n')) (f p)) then p else (S n')
-                                                             end.
-
-Theorem argMax_correct :
-  forall (f : nat -> Rat)(n : nat),
-    (forall n', (n' <= n)%nat -> (f n') <= f (argMax f n)).
-
-  induction n; intuition; simpl in *.
-  assert (n' = O) by omega; subst.
-  intuition.
-  destruct (eq_nat_dec n' (S n)).
-  subst.
-  destruct (le_Rat_dec (f0 (S n)) (f0 (argMax f0 n)));
-  intuition.
-
-  assert (n' <= n)%nat by omega.
-  destruct (le_Rat_dec (f0 (S n)) (f0 (argMax f0 n))).
-  eapply IHn; eauto.
-  eapply leRat_trans.
-  eapply IHn.
-  trivial.
-  eapply gtRat_impl_leRat; eauto.
-Qed.
-
-Theorem PRF_Advantage_max_exists :
-  forall i,
-      (i <= numCalls)%nat ->
-      PRF_Advantage_Game i <= PRF_Advantage_Game (argMax PRF_Advantage_Game numCalls).
-
-  intuition.
-  apply argMax_correct; trivial.
-
-Qed.
-
-(* The theorem above can be used in some of the arguments below, replacing 0 with (argMax PRF_Advantage_Game numCalls *)
-
 
 (* Lemma PRF_Advantages_lte : forall (i : nat), exists (j : nat), *)
 (*     PRF_Advantage_Game i <= PRF_Advantage_Game j. *)
@@ -2018,80 +2020,8 @@ Definition Gi_rf_dups_bad (i : nat) : Comp (bool * bool) :=
   [b, state] <-$2 PRF_Adversary i _ _ randomFunc_withDups nil;
   ret (b, hasInputDups state). 
 
-Theorem oracleCompMap_inner_oracle_equiv : 
-    forall (A B C D S : Set) (eqdc : EqDec C)(eqdd : EqDec D)(eqds : EqDec S) blocks (inv : S -> S -> Prop) (oc : nat * KV -> A -> OracleComp B C (D * (nat * KV))) s (o1 o2 : S -> B -> Comp (C * S)) s1 s2,
-    (forall s1 s2, inv s1 s2 -> (forall a, comp_spec (fun x1 x2 => (fst x1 = fst x2) /\ inv (snd x1) (snd x2)) (o1 s1 a) (o2 s2 a))) ->
-    inv s1 s2 ->
-    comp_spec (fun x1 x2 => fst x1 = fst x2 /\ inv (snd x1) (snd x2))
-   ((oracleCompMap_inner _ _ oc
-         s blocks) _ _
-        o1 s1)
-  ((oracleCompMap_inner _ _ oc
-         s blocks) _ _
-        o2 s2).
-  
-  induction blocks; intuition; simpl; fcf_simp.
-  apply comp_spec_ret; intuition.
-
-  fcf_simp.
-  fcf_skip.
-  eapply oc_comp_spec_eq.
-  apply H0.
-  intuition.
-  
-  fcf_simp.
-  simpl in *.
-  intuition.
-  pairInv.
-  fcf_skip.
-  simpl in *.
-  destruct b3.
-  simpl in *. subst.
-  fcf_simp.
-  apply comp_spec_ret.
-  simpl.
-  intuition.
-
-Qed.
-
-
-Theorem randomFunc_withDups_spec : 
-  forall s1 s2 a,
-  (forall a, arrayLookup _ s1 a = arrayLookup _ s2 a) ->
-  comp_spec
-     (fun x1 x2 : Bvector eta * list (Blist * Bvector eta) =>
-      fst x1 = fst x2 /\
-      (forall a0, 
-       arrayLookup _ (snd x1) a0 = arrayLookup _ (snd x2) a0))
-     (randomFunc ({ 0 , 1 }^eta) _ s1 a) (randomFunc_withDups s2 a).
-
-  intuition.
-  unfold randomFunc_withDups, randomFunc.
-  case_eq (arrayLookup eqdbl s1 a); intuition.
-  rewrite <- H.  
-  rewrite H0.
-  fcf_simp.
-  apply comp_spec_ret.
-  intuition.
-  simpl.
-  case_eq (a0 ?= a); intuition.
-  rewrite eqb_leibniz in H1.
-  subst. trivial.
-
-  rewrite <- H.
-  rewrite H0.
-  fcf_skip.
-  apply oneVector.
-  apply oneVector.
-  eapply comp_spec_ret.
-  intuition.
-  simpl.
-  rewrite H. 
-  trivial.
-Qed.
-
 Lemma oracleCompMap_rf_oracle_irrelevance : forall blocks calls i k v state,
-   comp_spec (fun x1 x2 => fst x1 = fst x2 /\ forall a, arrayLookup _ (snd x1) a = arrayLookup _ (snd x2) a)
+   comp_spec eq
      ((oracleCompMap_inner
          (pair_EqDec (list_EqDec (list_EqDec eqdbv))
             (pair_EqDec nat_EqDec eqDecState))
@@ -2106,13 +2036,32 @@ Lemma oracleCompMap_rf_oracle_irrelevance : forall blocks calls i k v state,
          (calls, (k, v)) blocks) (list (Blist * Bvector eta))
         (list_EqDec (pair_EqDec eqdbl eqdbv)) randomFunc_withDups state).
 Proof.
-  intros.
-  eapply comp_spec_consequence.
-  eapply (oracleCompMap_inner_oracle_equiv _ _ (fun s1 s2 => forall a, arrayLookup _ s1 a = arrayLookup _ s2 a)); intuition.
-  apply randomFunc_withDups_spec; intuition.
-  intuition.
+  induction blocks as [ | block blocks']; intros.
+  - simplify. fcf_spec_ret.
+  - simplify. fcf_skip_eq; kv_exist.
+    {
+      destruct (beq_nat calls 0).
+      + destruct (lt_dec calls i); repeat (simplify; fcf_skip_eq; kv_exist; simplify). fcf_spec_ret.
+        admit.
+        SearchAbout randomFunc_withDups.
+        (* TODO import that fn from PRF_DRBG instead and weaken precondition for randomFunc_withDups_spec *)
+        admit. (* didn't adam prove this? *)
+      + destruct (lt_dec calls i); repeat (simplify; fcf_skip_eq; kv_exist; simplify). fcf_spec_ret.
+        destruct (beq_nat calls i); repeat (simplify; fcf_skip_eq; kv_exist; simplify).
+        admit.
+        admit.
+        admit.
+
+        unfold GenUpdate_PRF_oc.
+        fcf_inline_first.
+        simplify.
+        fcf_spec_ret.
+    }
+    simplify. destruct b0.
+    fcf_skip_eq; kv_exist.
+    simplify. fcf_spec_ret.
 Qed.
- 
+
 Lemma Gi_rf_dups_return_bad_eq : forall (i : nat),
     Pr[x <-$ Gi_rf_bad i; ret fst x] == Pr[x <-$ Gi_rf_dups_bad i; ret fst x].
 Proof.
@@ -2120,15 +2069,8 @@ Proof.
   fcf_to_prhl_eq.
   unfold Gi_rf_bad.
   unfold Gi_rf_dups_bad.
-
-  repeat (simplify; fcf_skip).
+  repeat (simplify; fcf_skip_eq).
   apply oracleCompMap_rf_oracle_irrelevance.
-  simpl in *.
-  intuition; pairInv.
-  eapply comp_spec_eq_refl.
-  fcf_simp.
-  subst.
-  reflexivity.
 Qed.
 
 (* expose the bad event (dups) *)
@@ -2811,6 +2753,7 @@ Proof.
   }
 
   fcf_skip. instantiate (1 := (fun x y => fst x = fst y)).
+(*LENB AGAIN, some varibales not in scope*)
   apply Gen_loop_oc_states_diff.
 
   simplify. unfold rb_oracle. simplify. fcf_skip_eq. simplify. simpl in *. inversion H2. subst.
@@ -3340,8 +3283,6 @@ Proof.
 
         simplify.
         fcf_skip_eq; kv_exist.
-        simplify.
-        fcf_spec_ret.
       }
 
       (* END SWAP PROOF *)
@@ -4339,90 +4280,6 @@ note i only have to relate them on calls=i   *)
 
 (* ----------------------- *Identical until bad section *)
 
-Theorem Gen_loop_rb_intermediate_wf:
-  forall a b c,
-     well_formed_comp (Gen_loop_rb_intermediate b c a).
-
-  induction a; intuition; simpl; fcf_well_formed.
-
-Qed.
-
-Theorem GenUpdate_rb_intermediate_oc_wf :
-  forall b a,
-    well_formed_oc (GenUpdate_rb_intermediate_oc b a).
-
-    intros.
-    unfold GenUpdate_rb_intermediate_oc.
-    fcf_simp.
-    fcf_well_formed.
-    apply Gen_loop_rb_intermediate_wf.
-Qed.
-
-Theorem Gen_loop_oc_wf : 
-  forall a b0,
-     well_formed_oc (Gen_loop_oc b0 a).
-
-  induction a; intuition; simpl; fcf_well_formed.
-Qed.
-
-Theorem GenUpdate_noV_oc_wf : 
-  forall b a,
-    well_formed_oc (GenUpdate_noV_oc b a).
-
-  intros.
-  unfold GenUpdate_noV_oc.
-  fcf_simp.
-  fcf_well_formed.
-  apply Gen_loop_oc_wf.
-
-Qed.
-
-Theorem GenUpdate_oc_wf : 
-  forall b a,
-     well_formed_oc (GenUpdate_oc b a).
-
-  intros.
-  unfold GenUpdate_oc.
-  fcf_simp.
-  fcf_well_formed.
-  apply Gen_loop_oc_wf.
-Qed.
-
-Theorem GenUpdate_PRF_oc_wf : 
-  forall b a,
-     well_formed_oc (GenUpdate_PRF_oc b a).
-
-  intros.
-  unfold GenUpdate_PRF_oc.
-  fcf_simp.
-  fcf_well_formed.
-
-Qed.
-
-Theorem oracleCompMap_inner_wf : 
-  forall inputs s i,
-  well_formed_oc
-     (oracleCompMap_inner
-        (pair_EqDec (list_EqDec (list_EqDec eqdbv))
-           (pair_EqDec nat_EqDec eqDecState))
-        (list_EqDec (list_EqDec eqdbv)) (Oi_oc' i) 
-        s inputs).
-
-  induction inputs; intuition; simpl;
-  fcf_well_formed.
-  destruct (lt_dec a0 i).
-  apply GenUpdate_rb_intermediate_oc_wf.
-  
-  destruct (beq_nat a0 0).
-  apply GenUpdate_noV_oc_wf.
-  destruct (beq_nat a0 i).
-  apply GenUpdate_oc_wf.
-  eapply GenUpdate_PRF_oc_wf.
-
-Qed.
-
-
-
 (* SAME PROOF AS PRF_A_randomFunc_eq_until_bad (with the computation order switched) *)
 Theorem oracleCompMap__oracle_eq_until_bad_dups : forall (i : nat) b b0,
     comp_spec
@@ -4459,9 +4316,10 @@ Proof.
             (fun x => hasDups _ (fst (split x)))
             (fun x => hasDups _ (fst (split x))) eq); intuition.
 
-  - fcf_well_formed. 
-  apply oracleCompMap_inner_wf.
-
+  - fcf_well_formed. (* TODO hole: prove entire oraclecompmap is well_formed (how?) *)
+    SearchAbout well_formed_oc.
+    (* unfold well_formed_oc. *)
+    admit.
   - intros. unfold rb_oracle. fcf_well_formed.
   - intros. unfold randomFunc_withDups. destruct (arrayLookup eqdbl a b1); fcf_well_formed.
   - 
@@ -4989,8 +4847,8 @@ Definition Gi_rb_bad_map_no_keyinput : Comp bool :=
 (* v is randomly sampled here... but sometimes it's fixed (as in PRF_DRBG)? TODO *)
 (* seems too simple *)
 Definition Gi_rb_bad_map_inline_v : Comp bool :=
-  bits <-$ compMap eqdbv (fun _ => {0,1}^eta) (forNats (S blocksPerCall)); 
-  ret (hasDups eqdbv bits).
+  bits <-$ compMap (Bvector_EqDec eta) (fun _ => {0,1}^eta) (forNats (S blocksPerCall)); 
+  ret (hasDups (Bvector_EqDec eta) bits).
 
 Opaque hasDups.
 (* some of these inlinings can probably be done better in a different order or simultaneously *)
@@ -5029,17 +4887,16 @@ Qed.
 (*---------- Gi_rb_bad_eq_2 (splitting out `i`th call) *)
 Open Scope nat.
 
-Lemma split_out_oracle_call : forall (listLen : nat) (k v k1 v1 : Bvector eta) (callsSoFar i : nat)
-                                     (init : list (Blist * Bvector eta)),
-   callsSoFar <= i ->
-   listLen > 0 ->
+Lemma split_out_oracle_call : forall (nCalls : nat) (k v : Bvector eta) (calls i : nat) (init : list (Blist * Bvector eta)),
+   calls <= i ->
+   nCalls > 0 ->
    comp_spec eq
      (a <-$
       (oracleCompMap_inner
          (pair_EqDec (list_EqDec (list_EqDec eqdbv))
             (pair_EqDec nat_EqDec eqDecState))
          (list_EqDec (list_EqDec eqdbv)) (Oi_oc' i) 
-         (callsSoFar, (k, v)) (replicate listLen blocksPerCall)) (list (Blist * Bvector eta))
+         (calls, (k, v)) (replicate nCalls blocksPerCall)) (list (Blist * Bvector eta))
         (list_EqDec (pair_EqDec eqdbl eqdbv)) rb_oracle init;
       a0 <-$
       ([z, s']<-2 a;
@@ -5048,290 +4905,39 @@ Lemma split_out_oracle_call : forall (listLen : nat) (k v k1 v1 : Bvector eta) (
       z <-$ ([z, s']<-2 a0; x <-$ ret z; ret (x, s'));
       [_, state]<-2 z; ret hasInputDups state)
      (z <-$
-      (GenUpdate_oc (k1, v1) blocksPerCall) (list (Blist * Bvector eta))
+      (GenUpdate_oc (k, v) blocksPerCall) (list (Blist * Bvector eta))
         (list_EqDec (pair_EqDec eqdbl eqdbv)) rb_oracle init;
       [_, state]<-2 z; ret hasInputDups state).
 Proof.
-  induction listLen as [ | listLen']; intros; rename H into calls_leq_i.
-  (* listLen cannot be 0 *)
+  destruct nCalls as [ | nCalls']; intros; rename H into calls_leq_i.
+  (* nCalls > 0 *)
   - omega.
   (* first call *)
-  - Opaque Oi_oc'. Opaque GenUpdate_oc. 
+  - Opaque Oi_oc'. Opaque GenUpdate_oc. simplify.
+    assert (Hcalls : calls < i \/ calls = i) by omega.
+    destruct Hcalls.
     (* either calls < i or calls = i *)
-    remember (S listLen') as listLen.
-    (* clear HeqlistLen. *)
+    (* if calls < i... then the one call doesn't matter, and at some point calls = i, which reduces to the second case *)
+    (* need some kind of induction here? maybe *another* calls < i \/ calls = i? or just induct as-is? *)
 
-    assert (Hcalls : callsSoFar < i \/ callsSoFar = i) by omega.
-    destruct Hcalls as [ calls_lt_i | calls_eq_i ].
-    rewrite HeqlistLen.
+    (* if calls = i: then Oi_oc' i simplifies to GenUpdate_oc, and the states should be the same after. 
+       then need to deal with rest of calls: now calls > i. induct, and show that given the same starting rb_oracle state (right side empty), then for a subsequent call, the state doesn't change, so hasInputDups doesn't change ?
+ *)
+    
+    admit.
 
-    (* callsSoFar < i: deal with the first call, then apply IH, since callsSoFar < i -> S callsSoFar <= i *)
-    + simplify.
-      (* just simplify Oi_oc', don't skip *)
-      Transparent Oi_oc'.
-      simplify. destruct (lt_dec callsSoFar i) as [ calls_ltdec_i | calls_geqdec_i].
-      Focus 2. omega.
-      simplify.
-      fcf_irr_l. simplify.
-      fcf_irr_l. admit.
-      simplify.
+(* another induction? *)
 
-      Print Ltac rewrite_l.
-      Check comp_spec_eq_trans_l.
-      eapply comp_spec_eq_trans_l.
-      (* group first two lines *)
-      (* fcf_irr_l. admit. *)
-      (* simplify. *)
-      instantiate (1 := (a <-$
-                  (oracleCompMap_inner
-                     (pair_EqDec (list_EqDec (list_EqDec eqdbv))
-                        (pair_EqDec nat_EqDec eqDecState))
-                     (list_EqDec (list_EqDec eqdbv)) 
-                     (Oi_oc' i) (S callsSoFar, (k, b))
-                     (replicate listLen' blocksPerCall))
-                    (list (Blist * Bvector eta))
-                    (list_EqDec (pair_EqDec eqdbl eqdbv)) rb_oracle init;
-                  a0 <-$
-                  ([z, s']<-2 a;
-                   ([bits, _]<-2 z; $ ret bits) (list (Blist * Bvector eta))
-                     (list_EqDec (pair_EqDec eqdbl eqdbv)) rb_oracle s');
-                  z <-$ ([z, s']<-2 a0; x <-$ ret z; ret (x, s'));
-                  [_, state]<-2 z; ret hasInputDups state)).
-      { prog_equiv. fcf_spec_ret. }
+Admitted.
 
-      (* ugh, IH wants k and v to be the same, but they don't matter? should I generalize IH? *)
-      (* still need to get rid of list nonempty somehow? *)
-      eapply IHlistLen'. omega.
-      admit.
-
-
-    (* callsSoFar = i: then after the first call, S callsSoFar > i *)
-    (* apply separate lemma for calls = i, which inducts and applies another lemma for calls > i *)
-    + rewrite HeqlistLen.
-      simplify.
-      (* fcf_skip. *)
-      (* postcondition: (k,v) and init same afterward *)
-      (*  "(list (Bvector eta) * KV * list (Blist * Bvector eta))%type" with
- "(list (Bvector eta) * (nat * KV) * list (Blist * Bvector eta))%type". *)
-    (*   instantiate (1 := (fun x y => snd x = snd y (* oracle state eq *) *)
-    (*                                 /\ snd x = init (* and don't change *) *)
-    (*                                 /\ fst (fst x) = fst (fst y) (* sampled bits eq--doesn't matter though *) *)
-    (*                                 /\ snd (snd (fst x)) = snd (fst y) (* KV eq *) *)
-    (*                                 /\ fst (snd (fst x)) = S callsSoFar (* calls increases by 1 *) *)
-    (*               )). *)
-    (*   { admit. } *)
-
-    (*   simpl in *. breakdown H2. *)
-    (*   simplify. *)
-    (*   simpl in *. subst. *)
-    (* (* how can the IH work? there's no call on the right. I need a different induction--same as in calls > i, possibly *) *)
-    (*   destruct p as [bits [k' v']]. *)
-    (*   simplify. *)
-
-      (* generalized induction: calls (here = S i) > i -> init rb_oracle states same -> they remain the same *)
-      
-      admit.
-Qed.
-
-Open Scope nat.
-(* try split_out_oracle_call' without the nonempty hyp *)
-Lemma split_out_oracle_call_ind : forall (listLen : nat) (k v k1 v1 : Bvector eta) (callsSoFar i blocks : nat)
-                                     (init : list (Blist * Bvector eta)),
-    (* listLen > 0 -> *) (* attempt w/o this hypothesis *)
-    callsSoFar <= i ->
-  comp_spec eq
-     (a <-$
-      (oracleCompMap_inner
-         (pair_EqDec (list_EqDec (list_EqDec eqdbv))
-            (pair_EqDec nat_EqDec eqDecState))
-         (list_EqDec (list_EqDec eqdbv)) (Oi_oc' i) 
-         (callsSoFar, (k, v)) (replicate listLen blocks))
-        (list (Blist * Bvector eta)) (list_EqDec (pair_EqDec eqdbl eqdbv))
-        rb_oracle init;
-      a0 <-$
-      ([z, s']<-2 a;
-       ([bits, _]<-2 z; $ ret bits) (list (Blist * Bvector eta))
-         (list_EqDec (pair_EqDec eqdbl eqdbv)) rb_oracle s');
-      z <-$ ([z, s']<-2 a0; x <-$ ret z; ret (x, s'));
-      [_, state]<-2 z; ret hasInputDups state)
-     (if ge_dec i (listLen + callsSoFar) then (* the oracle is never used: i is past the end of the list *)
-        ret hasInputDups init
-      else if zerop i then      (* if the oracle is used and i = 0, then it's used in noV *)
-             (* I guess the v1 should really be whatever `v` the previous call changed it to, unless i=0, in which case, it should be the same v, but that's not inductive, ??????????? *)
-             (* or i can prove a hasDups-off-by-one result but that theorem needs a different form *)
-       (z <-$ (GenUpdate_noV_oc (k1, v1) blocks)
-              (list (Blist * Bvector eta)) (list_EqDec (pair_EqDec eqdbl eqdbv))
-              rb_oracle init;
-        [_, state]<-2 z;
-        ret hasInputDups state)
-      else                      (* if the oracle is used and i < numCalls, then it's used normally *)
-       (z <-$ (GenUpdate_oc (k1, v1) blocks)
-              (list (Blist * Bvector eta)) (list_EqDec (pair_EqDec eqdbl eqdbv))
-              rb_oracle init;
-        [_, state]<-2 z;
-        ret hasInputDups state)
-     ).
-Proof.
-  intros.
-  eapply comp_spec_eq_trans_r.
-  (* first, simplify two lines after ocm *)
-  instantiate (1 := (a <-$
-      (oracleCompMap_inner
-         (pair_EqDec (list_EqDec (list_EqDec eqdbv))
-            (pair_EqDec nat_EqDec eqDecState))
-         (list_EqDec (list_EqDec eqdbv)) (Oi_oc' i) 
-         (callsSoFar, (k, v)) (replicate listLen blocks))
-        (list (Blist * Bvector eta)) (list_EqDec (pair_EqDec eqdbl eqdbv))
-        rb_oracle init;
-      [_, s] <-2 a;
-      ret hasInputDups s)).
-  { prog_equiv. fcf_spec_ret. }
-  revert listLen k v k1 v1 callsSoFar i blocks init H.
-
-  induction listLen as [ | listLen']; intros.
-  (* base case: empty *)
-  - simplify.
-    destruct (ge_dec i callsSoFar). fcf_spec_ret.
-    omega.
-
-  (* inductive case *)
-  - Opaque Oi_oc'. Opaque GenUpdate_noV_oc. Opaque GenUpdate_oc.
-    rename H into calls_leq_i.
-    Opaque zerop.
-    simplify.
-    assert (calls_size : callsSoFar < i \/ callsSoFar = i) by omega.
-    destruct calls_size as [ calls_lt_i | calls_eq_i ].
-    (* callsSoFar < i -> after this call, S callsSoFar <= i *)
-    + (* is there some way to prove a postcondition on the left line only? want to show that rb_oracle's state doesn't change. *)
-      (* maybe equiv on left with a <-$ init? *)
-      (* also probably need to destruct stuff analogously to split_out_oracle_call'' *)
-      clear calls_leq_i.
-      Transparent Oi_oc'.
-      simplify.
-      (* clean up left side *)
-      destruct (lt_dec callsSoFar i). Focus 2. omega.
-      clear l.
-      (* fcf_irr_l. admit. simplify. destruct k0. *)
-      (* fcf_irr_l. admit. fcf_simp. simpl. fcf_simp. fcf_inline_first. *)
-      (* simplify. *)
-      (* strip off first call on left side, since it doesn't use the oracle *)
-      unfold GenUpdate_rb_intermediate_oc.
-      simplify.
-      fcf_irr_l. simplify.
-      fcf_irr_l. admit.
-      simplify.
-      rename b into v'.
-
-      eapply comp_spec_eq_trans_r.
-      instantiate (1 := (a <-$
-      (oracleCompMap_inner
-         (pair_EqDec (list_EqDec (list_EqDec eqdbv))
-            (pair_EqDec nat_EqDec eqDecState))
-         (list_EqDec (list_EqDec eqdbv)) (Oi_oc' i) 
-         (S callsSoFar, (k, v')) (replicate listLen' blocks))
-        (list (Blist * Bvector eta)) (list_EqDec (pair_EqDec eqdbl eqdbv))
-        rb_oracle init;
-      [_, s] <-2 a;
-      ret hasInputDups s)).
-      { prog_equiv. fcf_spec_ret. }
-      rewrite plus_n_Sm.
-      eapply IHlistLen'.
-      omega.
-
-    (* calls = i *)
-    + (* what's the form of the lemma i should apply here? *)
-      clear calls_leq_i.
-      (* here, the calls should both be skipped (since calls = i, the oracle is used) *)
-      (* then induct on the rest *)
-      Transparent Oi_oc'.
-      simplify.
-      subst.
-      (* clean up left side *)
-      destruct (lt_dec i i). omega.
-      (* clean up right side *)
-      destruct (ge_dec i (S (listLen' + i))). omega.
-
-      (* depends on whether i = 0, so destruct on that *)
-      destruct (zerop i) as [ i_eq_0 | i_gt_0 ].
-      (* i = 0 *)
-      { subst. simplify.
-        fcf_skip.
-        Transparent GenUpdate_noV_oc. 
-        instantiate (1 := (fun x y => snd x = snd y)).
-        { simplify. fcf_skip.
-          instantiate (1 := (fun x y => snd x = snd y)).
-          (* now we have a problem with Gen_loop_oc, where the first internal query may be different *)
-          Print Gen_loop_oc.
-          (* do we *have* to reason about every input? what about just the outputs? well, the next outputs depend on previous inputs but they're also independent of the input so that might work? *)
-          admit.
-
-          simplify. simpl in *. subst.
-          (* but now the oracle is queried with an output that differs... *)
-          fcf_skip_eq. admit.
-          simplify.
-          fcf_spec_ret. 
-        }
-        simplify.
-        (* prove the oracle is never used after this *)
-        (* what should the inductive condition be for "this"? *)
-        (* TODO apply lemma *)
-        (* i = 0, calls = 1 *)
-        destruct b0.
-        (* fcf_irr_l. simplify. *)
-        admit.
-      }
-      (* i <> 0 *)
-      { assert (i_neq_0 : i <> 0) by omega.
-        apply beq_nat_false_iff in i_neq_0.
-        rewrite i_neq_0.
-        pose proof (beq_nat_refl i) as i_refl.
-        rewrite <- i_refl.
-        clear i_neq_0 i_refl.
-        fcf_skip.
-        instantiate (1 := (fun x y => snd x = snd y)).
-        (* oh NO v and v1 are different, but we need to retain the fact that v and v1 are sampled from the same distribution... should (k,v) be same here? but they aren't same elsewhere for IH? oh NO, this feels like the other lemma all over again :( *)
-        (* wait what? the v are both sampled in beginning of GenUpdate_oc. it's GenUpdate_noV_oc that I have to worry about, because they were sampled from instantiate, whose information isn't retained here..... *)
-        (* wait, but the input v each time... is from the last call... i still need to worry about that :( *)
-        { Transparent GenUpdate_oc.
-          simplify.
-          fcf_skip_eq. unfold rb_oracle. fcf_skip_eq. fcf_spec_ret. repeat f_equal. admit.
-          fcf_skip_eq.
-          simplify.
-          fcf_skip_eq.
-          simplify.
-          fcf_spec_ret.
-        }
-        (* can they just start out with the same (k,v)...? would that break the IH? *)
-        simplify. destruct b0.
-        (* TODO apply lemma *)
-        eapply comp_spec_eq_trans_r.
-        (* simplify two lines after ocm *)
-        instantiate (1 :=  (a0 <-$
-      (oracleCompMap_inner
-         (pair_EqDec (list_EqDec (list_EqDec eqdbv))
-            (pair_EqDec nat_EqDec eqDecState))
-         (list_EqDec (list_EqDec eqdbv)) (Oi_oc' i) 
-         (S i, (b0, b1)) (replicate listLen' blocks))
-        (list (Blist * Bvector eta)) (list_EqDec (pair_EqDec eqdbl eqdbv))
-        rb_oracle b;
-        [_, b'] <-2 a0;
-        ret hasInputDups b')).
-        { prog_equiv. fcf_spec_ret. }
-        (* i = 0, calls = S i *)
-        admit.
-      }
-Qed.
-
-(* same goal as Gi_rb_bad_eq_2 *)
-Lemma eqt3 : forall k v i nCalls,
-    nCalls > 0 ->
+Lemma test_same_goal : forall (k v : Bvector eta) (i : nat),
    comp_spec eq
      (a <-$
       (oracleCompMap_inner
          (pair_EqDec (list_EqDec (list_EqDec eqdbv))
             (pair_EqDec nat_EqDec eqDecState))
          (list_EqDec (list_EqDec eqdbv)) (Oi_oc' i) 
-         (0%nat, (k, v)) (replicate nCalls blocksPerCall))
+         (0%nat, (k, v)) (replicate numCalls blocksPerCall))
         (list (Blist * Bvector eta)) (list_EqDec (pair_EqDec eqdbl eqdbv))
         rb_oracle nil;
       a0 <-$
@@ -5340,33 +4946,151 @@ Lemma eqt3 : forall k v i nCalls,
          (list_EqDec (pair_EqDec eqdbl eqdbv)) rb_oracle s');
       z <-$ ([z, s']<-2 a0; x <-$ ret z; ret (x, s'));
       [_, state]<-2 z; ret hasInputDups state)
-     (if ge_dec i nCalls then   (* if i >= numCalls, then the oracle is never used -> no dups *)
-        (ret false)
-      else if zerop i then      (* if the oracle is used and i = 0, then it's used in noV *)
-       (z <-$ (GenUpdate_noV_oc (k, v) blocksPerCall)
-              (list (Blist * Bvector eta)) (list_EqDec (pair_EqDec eqdbl eqdbv))
-              rb_oracle nil;
-        [_, state]<-2 z;
-        ret hasInputDups state)
-      else                      (* if the oracle is used and i < numCalls, then it's used normally *)
-       (z <-$ (GenUpdate_oc (k, v) blocksPerCall)
-              (list (Blist * Bvector eta)) (list_EqDec (pair_EqDec eqdbl eqdbv))
-              rb_oracle nil;
-        [_, state]<-2 z;
-        ret hasInputDups state)
-     ).
+     (z <-$
+      (GenUpdate_oc (k, v) blocksPerCall) (list (Blist * Bvector eta))
+        (list_EqDec (pair_EqDec eqdbl eqdbv)) rb_oracle (@nil (Blist * Bvector eta));
+      [_, state]<-2 z; ret hasInputDups state).
 Proof.
-  intros k v i nCalls nonempty.
-  Check compMap.
-  Print compMap.
-  (* apply split_out_oracle_call'; omega. *)
-(* TODO unify *)
-  admit.
+Admitted.
+
+Close Scope nat.
+
+Lemma eqt1 : forall k v,
+    comp_spec eq
+              (z <-$
+                 (GenUpdate_oc (k, v) blocksPerCall) (list (Blist * Bvector eta))
+                 (list_EqDec (pair_EqDec eqdbl eqdbv)) rb_oracle nil;
+               [_, state]<-2 z; ret hasInputDups state)
+     (z <-$
+      (GenUpdate_oc (k, v) blocksPerCall) (list (Blist * Bvector eta))
+        (list_EqDec (pair_EqDec eqdbl eqdbv)) rb_oracle nil;
+      [_, state]<-2 z; ret hasInputDups state).
+Proof.
+  intros.
+  assert (H :    comp_spec eq
+     (z <-$
+      (GenUpdate_oc (k, v) blocksPerCall) (list (Blist * Bvector eta))
+        (list_EqDec (pair_EqDec eqdbl eqdbv)) rb_oracle nil;
+      [_, state]<-2 z; ret hasInputDups state)
+     (z <-$
+      (GenUpdate_oc (k, v) blocksPerCall) (list (Blist * Bvector eta))
+        (list_EqDec (pair_EqDec eqdbl eqdbv)) rb_oracle nil;
+      [_, state]<-2 z; ret hasInputDups state)). { admit. }
+  apply H.                                                 
 Qed.
 
-(* ------- *)
-(* from eqt3 *)
-  (* apply split_out_oracle_call; omega. *)
+Lemma eqt2 : forall k v i,
+   comp_spec eq
+     (a <-$
+      (oracleCompMap_inner
+         (pair_EqDec (list_EqDec (list_EqDec eqdbv))
+            (pair_EqDec nat_EqDec eqDecState))
+         (list_EqDec (list_EqDec eqdbv)) (Oi_oc' i) 
+         (0%nat, (k, v)) (replicate numCalls blocksPerCall))
+        (list (Blist * Bvector eta)) (list_EqDec (pair_EqDec eqdbl eqdbv))
+        rb_oracle nil;
+      a0 <-$
+      ([z, s']<-2 a;
+       ([bits, _]<-2 z; $ ret bits) (list (Blist * Bvector eta))
+         (list_EqDec (pair_EqDec eqdbl eqdbv)) rb_oracle s');
+      z <-$ ([z, s']<-2 a0; x <-$ ret z; ret (x, s'));
+      [_, state]<-2 z; ret hasInputDups state)
+     (a <-$
+      (oracleCompMap_inner
+         (pair_EqDec (list_EqDec (list_EqDec eqdbv))
+            (pair_EqDec nat_EqDec eqDecState))
+         (list_EqDec (list_EqDec eqdbv)) (Oi_oc' i) 
+         (0%nat, (k, v)) (replicate numCalls blocksPerCall))
+        (list (Blist * Bvector eta)) (list_EqDec (pair_EqDec eqdbl eqdbv))
+        rb_oracle nil;
+      a0 <-$
+      ([z, s']<-2 a;
+       ([bits, _]<-2 z; $ ret bits) (list (Blist * Bvector eta))
+         (list_EqDec (pair_EqDec eqdbl eqdbv)) rb_oracle s');
+      z <-$ ([z, s']<-2 a0; x <-$ ret z; ret (x, s'));
+      [_, state]<-2 z; ret hasInputDups state).
+Proof.
+  intros.
+  assert (H :    comp_spec eq
+     (a <-$
+      (oracleCompMap_inner
+         (pair_EqDec (list_EqDec (list_EqDec eqdbv))
+            (pair_EqDec nat_EqDec eqDecState))
+         (list_EqDec (list_EqDec eqdbv)) (Oi_oc' i) 
+         (0%nat, (k, v)) (replicate numCalls blocksPerCall))
+        (list (Blist * Bvector eta)) (list_EqDec (pair_EqDec eqdbl eqdbv))
+        rb_oracle nil;
+      a0 <-$
+      ([z, s']<-2 a;
+       ([bits, _]<-2 z; $ ret bits) (list (Blist * Bvector eta))
+         (list_EqDec (pair_EqDec eqdbl eqdbv)) rb_oracle s');
+      z <-$ ([z, s']<-2 a0; x <-$ ret z; ret (x, s'));
+      [_, state]<-2 z; ret hasInputDups state)
+     (a <-$
+      (oracleCompMap_inner
+         (pair_EqDec (list_EqDec (list_EqDec eqdbv))
+            (pair_EqDec nat_EqDec eqDecState))
+         (list_EqDec (list_EqDec eqdbv)) (Oi_oc' i) 
+         (0%nat, (k, v)) (replicate numCalls blocksPerCall))
+        (list (Blist * Bvector eta)) (list_EqDec (pair_EqDec eqdbl eqdbv))
+        rb_oracle nil;
+      a0 <-$
+      ([z, s']<-2 a;
+       ([bits, _]<-2 z; $ ret bits) (list (Blist * Bvector eta))
+         (list_EqDec (pair_EqDec eqdbl eqdbv)) rb_oracle s');
+      z <-$ ([z, s']<-2 a0; x <-$ ret z; ret (x, s'));
+      [_, state]<-2 z; ret hasInputDups state)). { admit. }
+  apply H.
+Qed.                                                 
+
+(* Check eqdbv. *)
+(* Definition etn := 1%nat. *)
+(* Variable eqdbvn : EqDec (Bvector etn). *)
+
+Lemma eqt3 : forall k v i,
+   comp_spec eq
+     (a <-$
+      (oracleCompMap_inner
+         (pair_EqDec (list_EqDec (list_EqDec eqdbv))
+            (pair_EqDec nat_EqDec eqDecState))
+         (list_EqDec (list_EqDec eqdbv)) (Oi_oc' i) 
+         (0%nat, (k, v)) (replicate numCalls blocksPerCall))
+        (list (Blist * Bvector eta)) (list_EqDec (pair_EqDec eqdbl eqdbv))
+        rb_oracle nil;
+      a0 <-$
+      ([z, s']<-2 a;
+       ([bits, _]<-2 z; $ ret bits) (list (Blist * Bvector eta))
+         (list_EqDec (pair_EqDec eqdbl eqdbv)) rb_oracle s');
+      z <-$ ([z, s']<-2 a0; x <-$ ret z; ret (x, s'));
+      [_, state]<-2 z; ret hasInputDups state)
+     (z <-$
+      (GenUpdate_oc (k, v) blocksPerCall) (list (Blist * Bvector eta))
+        (list_EqDec (pair_EqDec eqdbl eqdbv)) rb_oracle nil;
+      [_, state]<-2 z; ret hasInputDups state).
+Proof.
+intros.
+assert (H :    comp_spec eq
+     (a <-$
+      (oracleCompMap_inner
+         (pair_EqDec (list_EqDec (list_EqDec eqdbv))
+            (pair_EqDec nat_EqDec eqDecState))
+         (list_EqDec (list_EqDec eqdbv)) (Oi_oc' i) 
+         (0%nat, (k, v)) (replicate numCalls blocksPerCall))
+        (list (Blist * Bvector eta)) (list_EqDec (pair_EqDec eqdbl eqdbv))
+        rb_oracle nil;
+      a0 <-$
+      ([z, s']<-2 a;
+       ([bits, _]<-2 z; $ ret bits) (list (Blist * Bvector eta))
+         (list_EqDec (pair_EqDec eqdbl eqdbv)) rb_oracle s');
+      z <-$ ([z, s']<-2 a0; x <-$ ret z; ret (x, s'));
+      [_, state]<-2 z; ret hasInputDups state)
+     (z <-$
+      (GenUpdate_oc (k, v) blocksPerCall) (list (Blist * Bvector eta))
+        (list_EqDec (pair_EqDec eqdbl eqdbv)) rb_oracle nil;
+      [_, state]<-2 z; ret hasInputDups state)).
+{ admit. }
+apply H.
+Qed.
 
 (* only the ith call with GenUpdate_oc (does it depend on what i is? casework on whether 0) ** hard *)
 Lemma Gi_rb_bad_eq_2 : forall (i : nat),
@@ -5390,14 +5114,11 @@ Proof.
   rename b into k. rename b0 into v.
   unfold maxCallsAndBlocks.
 
-Transparent eta.           (* *** TODO revert eta to a variable *)
-  (* apply eqt3. *)
-(* doesn't work but should *)
-
+  apply eqt3.
 (* Print Implicit split_out_oracle_call. *)
 
   assert (0 <= i)%nat by omega.
-  (* pose proof (@split_out_oracle_call numCalls k v 0%nat i nil H H_numCalls). *)
+  pose proof (@split_out_oracle_call numCalls k v 0%nat i nil H H_numCalls).
 
   (* Set Printing Implicit. *)
   (* eapply H0. *)
@@ -5407,6 +5128,82 @@ Transparent eta.           (* *** TODO revert eta to a variable *)
   (* pose proof (test_same_goal k v i). *)
   (* apply H.   *)
 
+  assert (test_same_goal' : 
+               comp_spec eq
+     (a <-$
+      (oracleCompMap_inner
+         (pair_EqDec (list_EqDec (list_EqDec eqdbvn))
+            (pair_EqDec nat_EqDec eqDecState))
+         (list_EqDec (list_EqDec eqdbvn)) (Oi_oc' i) 
+         (0%nat, (k, v)) (replicate numCalls blocksPerCall))
+        (list (Blist * Bvector etn)) (list_EqDec (pair_EqDec eqdbl eqdbvn))
+        rb_oracle nil;
+      a0 <-$
+      ([z, s']<-2 a;
+       ([bits, _]<-2 z; $ ret bits) (list (Blist * Bvector etn))
+         (list_EqDec (pair_EqDec eqdbl eqdbvn)) rb_oracle s');
+      z <-$ ([z, s']<-2 a0; x <-$ ret z; ret (x, s'));
+      [_, state]<-2 z; ret hasInputDups state)
+     (z <-$
+      (GenUpdate_oc (k, v) blocksPerCall) (list (Blist * Bvector etn))
+        (list_EqDec (pair_EqDec eqdbl eqdbvn)) rb_oracle nil;
+      [_, state]<-2 z; ret hasInputDups state) 
+).
+  { admit. }
+  assert (test_same_goal2 : 
+   @comp_spec bool bool bool_EqDec bool_EqDec (@eq bool)
+     (a <-$
+      (@oracleCompMap_inner nat (list (Bvector etn)) Blist 
+         (Bvector etn)
+         (@pair_EqDec (list (list (Bvector etn))) (nat * KV)
+            (@list_EqDec (list (Bvector etn))
+               (@list_EqDec (Bvector etn) eqdbvn))
+            (@pair_EqDec nat KV nat_EqDec eqDecState))
+         (@list_EqDec (list (Bvector etn)) (@list_EqDec (Bvector etn) eqdbvn))
+         (Oi_oc' i) (0%nat, (k, v)) (@replicate nat numCalls blocksPerCall))
+        (list (Blist * Bvector etn))
+        (@list_EqDec (Blist * Bvector etn)
+           (@pair_EqDec Blist (Bvector etn) eqdbl eqdbvn)) rb_oracle
+        (@nil (Blist * Bvector etn));
+      a0 <-$
+      ([z, s']<-2 a;
+       ([bits, _]<-2 z; $ ret bits) (list (Blist * Bvector etn))
+         (@list_EqDec (Blist * Bvector etn)
+            (@pair_EqDec Blist (Bvector etn) eqdbl eqdbvn)) rb_oracle s');
+      z <-$ ([z, s']<-2 a0; x <-$ ret z; ret (x, s'));
+      [_, state]<-2 z; ret hasInputDups state)
+     (z <-$
+      (GenUpdate_oc (k, v) blocksPerCall) (list (Blist * Bvector etn))
+        (@list_EqDec (Blist * Bvector etn)
+           (@pair_EqDec Blist (Bvector etn) eqdbl eqdbvn)) rb_oracle
+        (@nil (Blist * Bvector etn)); [_, state]<-2 z; ret hasInputDups state)).
+  { admit. }
+  Print Ltac fcf_to_prhl_eq.
+  Check comp_spec_eq_impl_eq.
+  eapply test_same_goal2.
+
+  (* Print Implicit test_same_goal. *)
+  eapply test_same_goal'.
+
+  Print Implicit (a <-$
+      (oracleCompMap_inner
+         (pair_EqDec (list_EqDec (list_EqDec eqdbvn))
+            (pair_EqDec nat_EqDec eqDecState))
+         (list_EqDec (list_EqDec eqdbvn)) (Oi_oc' i) 
+         (0%nat, (k, v)) (replicate numCalls blocksPerCall))
+        (list (Blist * Bvector etn)) (list_EqDec (pair_EqDec eqdbl eqdbvn))
+        rb_oracle nil;
+      a0 <-$
+      ([z, s']<-2 a;
+       ([bits, _]<-2 z; $ ret bits) (list (Blist * Bvector etn))
+         (list_EqDec (pair_EqDec eqdbl eqdbvn)) rb_oracle s');
+      z <-$ ([z, s']<-2 a0; x <-$ ret z; ret (x, s'));
+      [_, state]<-2 z; ret hasInputDups state)
+     (z <-$
+      (GenUpdate_oc (k, v) blocksPerCall) (list (Blist * Bvector etn))
+        (list_EqDec (pair_EqDec eqdbl eqdbvn)) rb_oracle nil;
+      [_, state]<-2 z; ret hasInputDups state).
+
   (* apply test_same_goal'. *)
   (* TODO unification error?? I can't apply split_out_oracle_call either :-/ *)
 
@@ -5414,13 +5211,15 @@ Transparent eta.           (* *** TODO revert eta to a variable *)
   (* Want to prove: the probability of duplicates in the state is the same for both games. How should I prove that? *)
   (* Do the k and v matter? They shouldn't, because the oracle has been replaced with RB. But could there be skipping problems?? *)
   (* Should I do casework on `i`? What else can I do casework or induction on? Maybe induct on a list (the generalized maxCallsAndBlocks), with calls < i? (currently it is 0) and there would be casework on calls < i, calls = i, calls > i. ok, so i should generalize, then add IH and induct on list, then case on i...? the structure is actually quite similar to the proofs i did before about the ith calls. *)
+  (* how to prototype this strategy and check if it will work? first, think through it on "paper" *)
+  (*  *)
   
   (* unfold oracleCompMap_inner. *)
   Transparent Oi_oc'.
   unfold Oi_oc'.
+
   
 Admitted.
-Opaque eta.
 
 (* get rid of oracle computation, transform GenUpdate_oc to GenUpdate_rb_inputs with hasDups on key and Vs explicitly
  ** hard? *)
@@ -5554,857 +5353,37 @@ Proof.
 
 Admitted.
 
-(* ------- redo *)
-Close Scope nat.
-
-(* match the form in dupProb_const *)
-Definition compMap_v (ls : list nat) (v : Bvector eta) :=
-  x <-$ compMap _ (fun _ => {0,1}^eta) ls;
-  ret hasDups _ (v :: x).
-
-(* generalized version of case_on_i for induction hyp *)
-Definition case_on_i_gen (i listLen callsSoFar nblocks : nat) init (v : Bvector eta) := 
-  if ge_dec i (listLen + callsSoFar) then (ret (hasInputDups init))
-  (* i = 0, so the last v is not an input. this case is exactly equivalent to adam’s gen_loop *)
-  else if zerop i then (compMap_v (forNats (pred nblocks)) v)
-  else (compMap_v (forNats nblocks) v).
-
-Definition case_on_i (i ncalls nblocks : nat) (v : Bvector eta) := 
-  if ge_dec i ncalls then (ret false)
-  (* i = 0, so the last v is not an input. this case is exactly equivalent to adam’s gen_loop *)
-  else if zerop i then (compMap_v (forNats (pred nblocks)) v)
-  else (compMap_v (forNats nblocks) v).
-
-Open Scope nat.
-
-(* TODO split this out into a separate module (CompMap_v_equiv.v) *)
-(* Transparent hasDups. *)
-
-Require Import CompMap_v_equiv.
-
-Lemma simplify_hasDups : forall (listLen i callsSoFar blocks : nat) (k v : Bvector eta) (l : list (Bvector eta))
-                                rb_state1,
-  comp_spec eq
-     (a <-$
-      (oracleCompMap_inner
-         (pair_EqDec (list_EqDec (list_EqDec (Bvector_EqDec eta)))
-            (pair_EqDec nat_EqDec eqDecState))
-         (list_EqDec (list_EqDec (Bvector_EqDec eta)))
-         (Oi_oc' i) (callsSoFar, (k, v))
-         (replicate listLen blocks)) (list (Blist * Bvector eta))
-        (list_EqDec (pair_EqDec eqdbl (Bvector_EqDec eta))) rb_oracle rb_state1;
-      a0 <-$
-      ([z, s']<-2 a;
-       ([resList, state'']<-2 z; $ ret (l :: resList, state''))
-         (list (Blist * Bvector eta))
-         (list_EqDec (pair_EqDec eqdbl (Bvector_EqDec eta))) rb_oracle s');
-      [_, rb_state2]<-2 a0; ret hasInputDups rb_state2)
-     (a <-$
-      (oracleCompMap_inner
-         (pair_EqDec (list_EqDec (list_EqDec (Bvector_EqDec eta)))
-            (pair_EqDec nat_EqDec eqDecState))
-         (list_EqDec (list_EqDec (Bvector_EqDec eta)))
-         (Oi_oc' i) (callsSoFar, (k, v))
-         (replicate listLen blocks)) (list (Blist * Bvector eta))
-        (list_EqDec (pair_EqDec eqdbl (Bvector_EqDec eta))) rb_oracle rb_state1;
-      [_, rb_state2] <-2 a;
-      ret hasInputDups rb_state2).
-Proof. intros. prog_equiv. fcf_spec_ret. Qed.
-
-Lemma rb_oracle_state_same_after_i : forall (listLen i callsSoFar blocks : nat) (k v : Bvector eta) left_state,
-   callsSoFar > i ->
-   comp_spec eq
-     (a0 <-$
-      (oracleCompMap_inner
-         (pair_EqDec (list_EqDec (list_EqDec (Bvector_EqDec eta)))
-            (pair_EqDec nat_EqDec eqDecState))
-         (list_EqDec (list_EqDec (Bvector_EqDec eta))) 
-         (Oi_oc' i) (callsSoFar, (k, v)) (replicate listLen blocks))
-        (list (Blist * Bvector eta))
-        (list_EqDec (pair_EqDec eqdbl (Bvector_EqDec eta))) rb_oracle
-        left_state;
-      [_, left_state']<-2 a0; ret hasInputDups left_state')
-     (ret hasInputDups left_state).
-Proof.
-  induction listLen as [ | listLen']; intros; rename H into calls_gt_i.
-  - simplify. fcf_spec_ret.
-  - simplify.
-    destruct (lt_dec callsSoFar i). omega.
-    assert (nonzero : callsSoFar <> 0) by omega.
-    apply beq_nat_false_iff in nonzero.
-    rewrite nonzero.
-    assert (neq_i : callsSoFar <> i) by omega.
-    apply beq_nat_false_iff in neq_i.
-    rewrite neq_i.
-    simplify.
-    
-    eapply comp_spec_eq_trans_r.
-    apply simplify_hasDups.
-    eapply comp_spec_eq_trans_r.
-    eapply IHlistLen'.
-    omega. fcf_spec_ret.
-Qed.
-
-(* --- try to get rid of oracle first *)
-
-Definition Gi_rb_bad_no_oracle' (k v : Bvector eta) (blocks : nat) : Comp bool :=
-  [bits, kv_state, otherInputs] <-$3 GenUpdate_rb_inputs (k, v) blocks;
-  [v', keyInput] <-2 otherInputs;
-  let firstInput := to_list v in (* fixed *)
-  let nextInput := to_list v' in (* extra input to refresh the v *)
-  let outputsAsInputs := firstn (blocksPerCall - 1) (map (fun v => to_list v) bits) in (* only the outputs (so v' is not duplicated) -- we need to remove the last output because that isn't used as an input. OR we can leave it in and get a slightly worse bound. *)
-  ret (hasDups _ (keyInput :: firstInput :: nextInput :: outputsAsInputs)).
-
-Import Permutation.
-
-(* matching PRF_DRBG_f_bad but returning the last result. ok if that's a bvector eta? *)
-Fixpoint Gen_loop_rb_blist (v : Bvector eta) (n : nat)
-  : Comp (list Blist * Bvector eta) := 
-  match n with
-  | O => ret (nil, v)
-  | S n' =>
-    v' <-$ {0,1}^eta;
-    [bits, v''] <-$2 Gen_loop_rb_blist v' n';
-    ret (to_list v' :: bits, v'')
-  end.
-
-(* emulates PRF_DRBG_f_bad_spec *)
-Theorem PRF_DRBG_f_bad_spec_withv : forall n v (ls : list (Blist * Bvector eta)),
-
-    comp_spec (fun (x1 : list (Bvector eta) * Bvector eta * list (Blist * Bvector eta)) (x2 : list Blist * Bvector eta) =>
-                  Permutation (fst (split (snd x1))) ((fst (split ls)) ++ fst x2))
-
-              (* TODO need to prove output keys eq? *)
-   (* comp_spec *)
-   (*   (fun (x : list (Bvector eta) * Bvector eta * list (Blist * Bvector eta)) *)
-   (*      (y : list (Bvector eta) * Bvector eta) => fst x = y /\ True) *)
-
-     (* ((PRF_DRBG_f_G2 v n) _ _ *)
-     (*    (fun (ls : list (D * Bvector eta)) (a : D) => *)
-     (*     x <-$ { 0 , 1 }^eta; ret (x, (a, x) :: ls)) *)
-     (*    ls) *)
-     ((Gen_loop_oc v n) (list (Blist * Bvector eta))
-        (list_EqDec (pair_EqDec eqdbl (Bvector_EqDec eta)))
-        (fun (state : list (Blist * Bvector eta)) (input : Blist) =>
-         output <-$ { 0 , 1 }^eta; ret (output, (input, output) :: state)) ls)
-        (* ((to_list v, a) :: init)) *)
-
-     (* (PRF_DRBG_f_bad v n). *)
-     (Gen_loop_rb_blist v n).
-Proof.
-  induction n; intuition; simpl in *.
-  fcf_simp.
-  fcf_spec_ret.
-  simpl.
-  rewrite app_nil_r.
-  apply Permutation_refl.
-
-  fcf_inline_first.
-  fcf_skip.
-  fcf_skip.
-  fcf_simp.
-  fcf_spec_ret.
-  simpl in H4.
-  simpl.
-  destruct (split ls).
-  simpl in H4. simpl.
-  (* wait, the two of them are defined totally differently... gen_loop_rb_blist and prf_drbg_f_bad *)
-  eapply Permutation_trans.
-  apply H4.
-  (* apply Permutation_cons_app. *)
-  (* apply Permutation_refl. *)
-Admitted.
-
-Lemma Gi_rb_collisions_remove_oracle_first : forall k v blocks init,
-  comp_spec eq
-     (a <-$
-      (GenUpdate_oc (k, v) blocks) (list (Blist * Bvector eta))
-        (list_EqDec (pair_EqDec eqdbl (Bvector_EqDec eta))) rb_oracle init;
-      [_, init']<-2 a; ret hasInputDups init') 
-     (Gi_rb_bad_no_oracle' k v blocks).
-Proof.
-  intros k v blocks init.
-  unfold GenUpdate_oc.
-  unfold Gi_rb_bad_no_oracle'. simplify.
-  unfold rb_oracle. simplify.
-  fcf_skip_eq.
-  simplify.
-  (* Error: Impossible to unify "(list (Bvector eta) * Bvector eta)%type" with
- "(list (Bvector eta) * Bvector eta * list (Blist * Bvector eta))%type". *)
-  fcf_skip.
-  (* instantiate (1 := (fun x y => fst (split (snd x)) = map (fun c  => to_list c) (fst y))). *)
-  instantiate (1 := (fun x y => fst x = y /\ True)).
-  {
-    Print Gen_loop_rb_intermediate.
-    revert k v blocks init a. clear H.
-    induction blocks as [ | blocks']; intros; simplify.
-    (* need to generalize RB state? *)
-    - fcf_spec_ret.
-    (* - fcf_skip_eq. fcf_skip. (* eapply IHblocks'. *) *)
-    - admit.
-  }
-  simpl in *. 
-  simplify.
-  fcf_skip_eq.
-  simplify.
-  inversion H3. subst.
-  fcf_spec_ret.
-  unfold hasInputDups. simpl. 
-  unfold split. 
-  simplify.                     (* why doesn't simpl work... *)
-  apply Permutation_hasDups.
-  constructor.
-
-  (* can I prove the two postconditions separately and then conjoin them?? *)
-  SearchAbout (comp_spec (fun x y => _ /\ _) _ _).
-  (* TODO make it generic *)
-  assert (comp_spec_and : forall P Q a b, comp_spec P a b -> comp_spec Q a b -> comp_spec (fun c d => P c d /\ Q c d) a b).
-  { intros. admit. }
-    
-
-  admit.
-  (* don't do f_equal, we want to apply Permutation_hasDups *)
-  (* Transparent hasDups. *)
-  (* remember (to_list v *)
-  (*        :: to_list a *)
-  (*           :: firstn (blocksPerCall - 1) *)
-  (*                (map (fun v0 : Vector.t bool eta => to_list v0) l)) as inner. *)
-  (* simpl. *)
-  (* f_equal. f_equal. *)
-
-  (* i can't use PRF_DRBG_f_G2 as-is because it doesn't return the last bitvector, and i need the last bitvector as the k input? or could i replace it with anything? *)
-  (* also injD is to_list *)
-
-Print rb_oracle.
-(* actually the order is wrong... rb_oracle conses each new query into the beginning *)
-(* it should be (rev firstn map to_list l) ++ [to_list a] ++ [to_list v] *)
-(* or maybe i should reason about permutations... *)
-(* also, yeah, i need to add rb_oracle state to the postcondition for loop *)
-(* also, if i prove permutation here, will that allow me to prove eq later? probably yes, eq is on hasDups *)
-(* then I need to use a theorem on hasDups $ perm l = hasDups l *)
-(* can i apply PRF_DRBG_f_bad_spec here?? and if I do, is that postcondition helpful? and can I directly apply it, or do I need to copy-and-paste the proof? *)
-
-  (* v = the input v, a = output of rb_oracle v *)
-  (* the `to_list v` got stuck in the rb_oracle's input state in gen_loop_oc *)
-(* this should be the postcondition!... is it true? what happened to my actual postcondition? *)
-  (* the second half worked (the last v that each loop is the output to each k-sampling) *)
-  (* the first half was thrown away (hasInputDups ignores the bits output) *)
-Qed.
-
-(* --- *)
-
-(* maybe I should remove k entirely? *)
-Definition GenUpdate_oc_noKsample (state : KV) (n : nat) :
-  OracleComp (list bool) (Bvector eta) (list (Bvector eta) * KV) :=
-  [k, v_0] <-2 state;
-  v <--$ (OC_Query _ (to_list v_0)); (* ORACLE USE *)
-  [bits, v'] <--$2 Gen_loop_oc v n;
-  $ ret (bits, (k, v')).
-
-(* try removing k first, but i lose information about the length of the list... *)
-Lemma Gi_rb_collisions_remove_k_first : forall k v blocks init,
-  comp_spec eq
-     (a <-$
-      (GenUpdate_oc (k, v) blocks) (list (Blist * Bvector eta))
-        (list_EqDec (pair_EqDec eqdbl (Bvector_EqDec eta))) rb_oracle init;
-      [_, init']<-2 a; ret hasInputDups init') 
-     (a <-$
-      (GenUpdate_oc_noKsample (k, v) blocks) (list (Blist * Bvector eta))
-        (list_EqDec (pair_EqDec eqdbl (Bvector_EqDec eta))) rb_oracle init;
-      [_, init']<-2 a; ret hasInputDups init').
-Proof.
-  intros k v blocks init.
-  unfold GenUpdate_oc.
-  unfold GenUpdate_oc_noKsample. simplify.
-  unfold rb_oracle. simplify.
-  fcf_skip_eq. simplify.
-  (* maybe prove something about gen_loop and how its output is eq to comp_map here? *)
-  (* or really, oracleCompMap... *)
-  (* proving a stronger postcondition than eq *)
-  (* eapply comp_spec_seq. apply true. apply true. *)
- (* instantiate (1 := (fun x y => x = y /\ True )). *)
-  (* admit. *)
-  (* reasoning about split of anything is annoying. maybe get rid of the outputs first/? *)
-  (* or: get rid of oracle, then prove that it's hasDups eqdbl keyInput :: map to_list compMap... *)
-SearchAbout Forall.
-Print GenUpdate_oc.
-
-  fcf_skip. simplify.
-  fcf_irr_l. simplify.
-  unfold hasInputDups.
-  simplify.
-  fcf_spec_ret.
-  Transparent hasDups. simplify.
-  (* uh oh, I lost information about all elements of l having the same length and b1 having the same length as them *)
-(* i have the `to_list b1` (now i need to reason about `Bvector eta`s??) *)
-(* maybe i want a postcondition on `l = map to_list ...` *)
-(* in that case, I should simplify gen_loop first *)
-(* there's to_list_length *)
-
-Admitted.
-
-Lemma Gi_rb_collisions_inner_eq : forall k v blocks init,
-  comp_spec eq
-     (a <-$
-      (GenUpdate_oc (k, v) blocks) (list (Blist * Bvector eta))
-        (list_EqDec (pair_EqDec eqdbl (Bvector_EqDec eta))) rb_oracle init;
-      [_, init']<-2 a; ret hasInputDups init') (compMap_v (forNats blocks) v).
-Proof.
-  intros k v blocks init.
-  unfold GenUpdate_oc.
-  unfold compMap_v.
-
-  (* why not get rid of the oracle computation in GenUpdate_oc? *)
-  Print Gi_rb_bad_no_oracle.
-  Print GenUpdate_rb_inputs.
-  (* i should also get rid of that key line ASAP, and convert everything to vectors *)
-  (* what about reasoning about permutations? *)
-
-  simplify.
-  Transparent compMap.
-  unfold rb_oracle. simplify.
-  fcf_irr_l.
-  (* maybe I don't want to simplify it all the way *)
-  (* fcf_simp. *)
-  simplify.
-  fcf_skip.
-(* or, rewrite left side with gen_loop first *)
-  (* I can essentially use Adam's proof here *)
-(* Check (fun x y => split (snd x) = map (fun c => to_list c) y). *)
-  instantiate (1 := (fun x y => map (fun c => fst c) (snd x) = map (fun c => to_list c) y)).
-  { admit. }
-(* again, this might not be very useful as a postcondition *)
-  simplify.
-  simpl in H3.
-  fcf_irr_l. simplify.
-  fcf_spec_ret.
-  unfold hasInputDups.
-  (* and it's annoying to compare lists to bvectors *)
-  simpl.
-(* where's b? *)
-
-Admitted.
-
-(* ------------ Adam's version of Gi_rb_collisions_inner_eq *)
-
-(* TODO see if I can prove a more general version of compmap_v_eq using compMap_v_eq_h *)
-(* From email: "See compMap_v_eq_h in the file I attached on Apr 22. I think this is what you want. Note that this fact only holds if v and w are both not in init (you can also prove it when both are in init by removing the compMap statements with fcc_irr). *)
-
-(* adding init on the right *)
-Opaque hasDups.
-Lemma Gi_rb_collisions_inner_eq_general : forall (blocks : nat) (k v : Bvector eta) (init : list (Blist * Bvector eta)),
-  comp_spec eq
-     (a <-$
-      (GenUpdate_oc (k, v) blocks) (list (Blist * Bvector eta))
-        (list_EqDec (pair_EqDec eqdbl (Bvector_EqDec eta))) rb_oracle init;
-      [_, init']<-2 a; ret hasInputDups init') 
-      (x <-$
-      compMap (Bvector_EqDec eta) (fun _ : nat => { 0 , 1 }^eta)
-        (forNats (S blocks)); 
-        ret hasDups _ ((map (@to_list _ _) (v :: x)) ++ (map (@fst _ _ ) init))).
-Proof.
-  intuition; simpl.
-  unfold rb_oracle.
-  fcf_inline_first.
-  fcf_skip. (* b here: maybe we just forgot to account for it in some postcondition? *)
-  rename b into v_update_output.
-  fcf_inline_first.
-  fcf_skip.
-  (* is (S blocks) really correct? it does make the proof more convenient *)
-
-  Theorem Gen_loop_oc_compMap_eq_no_v_init : forall blocks (v_init v_init_input : Bvector eta) init,
-    comp_spec
-      (* (fun a b => map (@fst _ _) (snd a) = (map (@to_list _ _ ) (v :: b)) ++ (map (@fst _ _) init)) *)
-
-      (* bits, last element of bits, and oracle state vs. just bits *)
-     (fun (loop_out : list (Bvector eta) * Bvector eta * list (Blist * Bvector eta))
-          (map_out : list (Bvector eta)) =>
-          map (fst (B:=Bvector eta)) (snd loop_out) =         (* inputs to oracle *)
-          map (to_list (n:=eta)) map_out ++ map (fst (B:=Bvector eta)) init)
-     (* existing first input + generated bits (as blist) + initial inputs *)
-
-     ((Gen_loop_oc v_init blocks) (list (Blist * Bvector eta)) (* NOTE: b is the initial input to Gen_loop_oc *)
-        (list_EqDec (pair_EqDec eqdbl (Bvector_EqDec eta)))
-        (fun (state : list (Blist * Bvector eta)) (input : Blist) =>
-         output <-$ { 0 , 1 }^eta; ret (output, (input, output) :: state))
-        init)
-
-     (compMap (Bvector_EqDec eta) (fun _ : nat => { 0 , 1 }^eta) (forNats blocks)).
-  Proof.
-    induction blocks as [ | blocks']; intuition; simpl in *.
-
-    - fcf_simp. fcf_spec_ret.
-    - fcf_inline_first.
-      fcf_irr_l.
-      simplify.
-      (* maybe you shouldn't be skipping? maybe it's the same problem as the earlier skip? *)
-      (* problem is that the right should map to the oracle's inputs, not outputs *)
-      fcf_skip.
-      rename b into sampled_v.
-      fcf_skip.
-      simpl in *.
-      fcf_spec_ret.
-      simpl.
-      rewrite H4.
-      rename a into loop_bits. rename b0 into last_loop_bits. rename b into end_loop_state.
-      rename b1 into map_bits.
-  (* the order is different *and* there's a difference between v_init and sampled_v *)
-  (* also can i even apply this in the larger theorem? *)
-  Admitted.
-
-  simpl.
-  apply Gen_loop_oc_compMap_eq_no_v_init. bv_exist.
-  simplify.
-  fcf_irr_l. rename a0 into key_output.
-  simpl in *.
-  simplify.
-  fcf_spec_ret.
-  unfold hasInputDups.
-  simpl.
-  remember (split b) as z. destruct z.
-  simpl.
-  rename b0 into key_input. rename l into oracle_inputs. rename b into oracle_state. rename l0 into oracle_outputs.
-  assert (split_map_fst : forall A B (l : list (A * B)), fst (split l) = map (@fst _ _) l).
-  { induction l as [ | x xs]; intros. simpl. reflexivity. simpl. destruct x.  simpl. destruct (split xs). simpl. simpl in *. subst. reflexivity. }
-
-  rewrite <- split_map_fst in H4.
-  rewrite <- Heqz in H4.
-  simpl in H4.
-  rewrite H4.
-
-  Transparent hasDups.
-  (* TODO: we need that hypothesis about init = to_list whatever (it doesn't matter b/c init is nil when we apply thm) *)
-  remember (map (to_list (n:=eta)) b1 ++
-         to_list v :: map (fst (B:=Bvector eta)) init) as rest.
-  (* rewrite app_comm_cons. *)
-  unfold hasDups at 1. fold hasDups.
-  Opaque hasDups.
-(* former: prove to_list key_input cannot be in the latter list *)
- (* there's still an extra v_update_output in the state, same as below--maybe we forgot it in a postcondition on the right? *)
-(* would it be a loop problem or a theorem statement problem? *)
-
-Admitted.
-
-Lemma Gi_rb_collisions_inner_eq_general_original : forall (blocks : nat) (k v : Bvector eta) (init : list (Blist * Bvector eta)),
-  comp_spec eq
-     (a <-$
-      (GenUpdate_oc (k, v) blocks) (list (Blist * Bvector eta))
-        (list_EqDec (pair_EqDec eqdbl (Bvector_EqDec eta))) rb_oracle init;
-      [_, init']<-2 a; ret hasInputDups init') 
-      (x <-$
-      compMap (Bvector_EqDec eta) (fun _ : nat => { 0 , 1 }^eta)
-        (forNats blocks); 
-        ret hasDups _ ((map (@to_list _ _) (v :: x)) ++ (map (@fst _ _ ) init))).
-Proof.
-  intuition; simpl.
-  unfold rb_oracle.
-  fcf_inline_first.
-  fcf_irr_l.
-  simplify.
-  (* fcf_skip. (* b here: maybe we just forgot to account for it in some postcondition? *) *)
-  rename a into v_update_output.
-  fcf_skip.
-  (* is (S blocks) really correct? it does make the proof more convenient *)
-
-  (* should `to_list v` be in the oracle state here? maybe if we generalized it to any init? *)
-  Theorem Gen_loop_oc_compMap_eq : forall blocks (v_update_output v_init_input : Bvector eta) init,
-    comp_spec
-      (* (fun a b => map (@fst _ _) (snd a) = (map (@to_list _ _ ) (v :: b)) ++ (map (@fst _ _) init)) *)
-
-      (* bits, last element of bits, and oracle state vs. just bits *)
-     (fun (loop_out : list (Bvector eta) * Bvector eta * list (Blist * Bvector eta))
-          (map_out : list (Bvector eta)) =>
-          map (fst (B:=Bvector eta)) (snd loop_out) =         (* inputs to oracle *)
-          to_list v_init_input :: map (to_list (n:=eta)) map_out ++ map (fst (B:=Bvector eta)) init)
-     (* maybe i need In v_update_output loop_out or alternatively the rightmost one should really exclude it due to adam's trick with the S ... *)
-     (* existing first input + generated bits (as blist) + initial inputs *)
-
-     ((Gen_loop_oc v_update_output blocks) (list (Blist * Bvector eta)) (* NOTE: b is the initial input to Gen_loop_oc *)
-        (list_EqDec (pair_EqDec eqdbl (Bvector_EqDec eta)))
-        (fun (state : list (Blist * Bvector eta)) (input : Blist) =>
-         output <-$ { 0 , 1 }^eta; ret (output, (input, output) :: state))
-        ((to_list v_init_input, v_update_output) :: init))
-
-     (compMap (Bvector_EqDec eta) (fun _ : nat => { 0 , 1 }^eta) (forNats blocks)).
-  Proof.
-    induction blocks as [ | blocks']; intuition; simpl in *.
-    - fcf_simp.
-      (* fcf_spec_ret. *)
-      eapply comp_spec_ret.
-      simpl.                    (* simplifies to `to_list v :: map fst init`. should it? it would work w/o to_list v? *)
-      reflexivity.
-
-    - fcf_inline_first.
-      fcf_skip.
-      rename b into sampled_v.
-      specialize (IHblocks' sampled_v v_update_output ((to_list v_init_input, v_update_output) :: init)).
-      (* IH works? what does the IH say? is the postcondition accounting for the new rb_state?*)
-      fcf_skip. apply IHblocks'.
-      simpl in *.
-      rename b1 into compMap_gen_bits.
-      rename a into loop_bits.
-      rename b0 into last_loop_v.
-      rename b into end_loop_state.
-      apply comp_spec_ret.
-      simpl.
-      rewrite H4.
-      (* it's mixing up v_update_output and sampled_v. why? *)
-      f_equal. admit.
-      (* oh there's more *)
-      admit.
-      (* the left and right don't look equal at all? removing the last list, *)
-      (* to_list v_init :: map to_list compmap_gen_bits ++ [to_list v_init_input] =
-         to_list v_init_input :: to_list sampled_v :: map to_list compmap_gen_bits *)
-      (* the order is wrong, and v_init != sampled_v. why is this problem arising? *)
-      (* maybe we need Permutation again *)
-      (* what would cause them to be in a different order? *)
-  (* what's causing this problem? is it the same as the problem I ran into earlier, due to how Gen_loop_oc is defined (which doesn't match the cons definition of Gen_loop)? *)
-
-  (* maybe running into that "different first list item" problem *)
-  Admitted.
-
-  apply Gen_loop_oc_compMap_eq.
-
-  fcf_simp.
-  simpl in *.
-
-  fcf_inline_first.
-  fcf_irr_l.
-  fcf_inline_first. 
-  eapply comp_spec_ret.
-  unfold hasInputDups.
-
-  simpl. remember (split b) as z. destruct z.
-
-  assert (split_map_fst : forall A B (l : list (A * B)), fst (split l) = map (@fst _ _) l).
-  { induction l1 as [ | x xs]; intros. simpl. reflexivity. simpl. destruct x.  simpl. destruct (split xs). simpl. simpl in *. subst. reflexivity. }
-
-  rewrite <- split_map_fst in H3.
-  rewrite <- Heqz in H3.
-  simpl in H3.
-  rewrite H3.
-  simpl.
-  (* well, getting rid of S on S blocks solved that problem--isn't this where I was before? *)
-  Transparent hasDups.
-  (* TODO: we need that hypothesis about init = to_list whatever (it doesn't matter b/c init is nil when we apply thm) *)
-  unfold hasDups at 1. fold hasDups.
-  Opaque hasDups.
-
-
-  (* rename b0 into rest_of_oracle_state. *)
-  (* rename a0 into key_output. *)
-  (* simpl. *)
-  (* remember (split rest_of_oracle_state) as z. *)
-  (* destruct z. *)
-
-  (* (* added *) *)
-  (* simpl. *)
-  (* rename b1 into key_input. *)
-  (* rename b2 into bits_list. *)
-  (* rename l into oracle_inputs. *)
-
-  (* ok, we now have to_list b1 ++ zeroes, should prove that is removable *)
-  (* using H4, why is there the extra `to_list b` on the right? otherwise, everything else matches *)
-  (* how to ue H4? *)
-
-  (* what/where is b0? *)
-  (* how to prove that "separate theorem" and what should the theorem statement be? *)
-  (* did we already use H4? it relates b0 to b2 and init, and Heqz (which we didn't actually use?) relates (l,l0) to b0 (which doesn't appear in the theorem statement)... *)
-  (* does adam mean H2 or H4? *)
-
-  (* From H2, we know that b is correctly related to b0. This can be proved in a separate theorem by induction on blocks *)
-  admit.
-(* ?? *)
-Qed.
-
-(* what is this other proof? *)
-(*  intros k v blocks init.
-  unfold GenUpdate_oc.
-  unfold compMap_v.
-
-  Print rb_oracle.
-
-  induction blocks; intuition; simpl in *.
-  fcf_inline_first.
-  fcf_irr_l.
-  admit.
-  repeat (fcf_inline_first; fcf_simp).
-  simpl.
-  fcf_inline_first.
-  fcf_irr_l.
-  admit.
-  repeat (fcf_inline_first; fcf_simp).
-  unfold rb_oracle in *.
-  repeat simp_in_support.
-  unfold hasInputDups.
-  simpl.
-  unfold compMap_v. simpl.
-Qed. *)
-
-(* ------------ end Adam's version of Gi_rb_collisions_inner_eq *)
-
-Lemma split_out_oracle_call_forall : 
-    forall (listLen : nat) (k v v_prev : Bvector eta) (callsSoFar i blocks : nat) (init : list (Blist * Bvector eta)),
-      callsSoFar <= i ->
-   comp_spec eq
-     (a <-$
-      (oracleCompMap_inner
-         (pair_EqDec (list_EqDec (list_EqDec (Bvector_EqDec eta)))
-            (pair_EqDec nat_EqDec eqDecState))
-         (list_EqDec (list_EqDec (Bvector_EqDec eta))) 
-         (Oi_oc' i) (callsSoFar, (k, v)) (replicate listLen blocks))
-        (list (Blist * Bvector eta))
-        (list_EqDec (pair_EqDec eqdbl (Bvector_EqDec eta))) rb_oracle init;
-      [_, state]<-2 a; ret hasInputDups state)
-     (case_on_i_gen i listLen callsSoFar blocks init v_prev).
-Proof.
-  unfold case_on_i_gen.
-  induction listLen as [ | listLen']; intros.
-
-   (* base case: empty *)
-  - simplify.
-    destruct (ge_dec i callsSoFar). { fcf_spec_ret. } { omega. }
-
-  (* inductive case *)
-  - Opaque Oi_oc'. Opaque GenUpdate_noV_oc. Opaque GenUpdate_oc.
-    rename H into calls_leq_i.
-    Opaque zerop.
-    simplify.
-    assert (calls_size : callsSoFar < i \/ callsSoFar = i) by omega.
-    destruct calls_size as [ calls_lt_i | calls_eq_i ].
-    (* callsSoFar < i -> after this call, S callsSoFar <= i *)
-    + clear calls_leq_i.
-      Transparent Oi_oc'.
-      simplify.
-
-      (* clean up left side *)
-      destruct (lt_dec callsSoFar i). Focus 2. omega.
-      clear l.
-
-      (* strip off first call on left side, since it doesn't use the oracle *)
-      unfold GenUpdate_rb_intermediate_oc.
-      simplify.
-      fcf_irr_l. simplify.
-      fcf_irr_l. admit. (* note the k doesn't change *)
-      simplify.
-      rename b into v'.
-
-      eapply comp_spec_eq_trans_r.
-      apply simplify_hasDups.
-      rewrite plus_n_Sm.
-      eapply IHlistLen'.
-      omega.
-
-    (* calls = i *)
-    + (* what's the form of the lemma i should apply here? *)
-      clear calls_leq_i.
-      (* here, the calls should both be skipped (since calls = i, the oracle is used) *)
-      (* then induct on the rest *)
-      Transparent Oi_oc'.
-      simplify.
-      subst.
-      (* clean up left side *)
-      destruct (lt_dec i i). omega.
-      (* clean up right side *)
-      destruct (ge_dec i (S (listLen' + i))). omega.
-
-      (* depends on whether i = 0, so destruct on that *)
-      destruct (zerop i) as [ i_eq_0 | i_gt_0 ].
-      (* i = 0 *)
-      {
-        subst. simplify.
-
-        (* replace v_prev with v, since the const vector in front doesn't matter *)
-        eapply comp_spec_eq_trans_r.
-        Focus 2.
-        eapply (compMap_v_eq (forNats (pred blocks)) v v_prev).
-        Check compMap_v_eq.
-        unfold compMap_v.
-
-        fcf_skip.
-        (* the types even differ here: Blist vs Bvector eta. is it easier to do to_list or from_list? *)
-        Print GenUpdate_noV_oc.
-        instantiate (1 := (fun x y => map (fun c => fst c) (snd x) = map (fun c => to_list c) y)).
-        { admit. }
-        (* is this postcondition (eq on blocks gen) too strong? or is it actually right? *)
-        (* where should the hasDups go? *)
-        (* should i prove hasDups on GenUpdate_noV_oc? rewrite *)
-
-        (* induction: prove the oracle is never used in subsequent calls *)
-        (* TODO apply lemma *)
-        (* i = 0, calls = 1 *)
-        simpl in *.
-        simplify.
-
-        (* why doesn't it unify? *)
-        (* eapply comp_spec_eq_trans_r. *)
-        (* eapply simplify_hasDups. *)
-        (* eapply comp_spec_eq_trans_r. *)
-        (* apply rb_oracle_state_same_after_i; omega. *)
-        (* fcf_irr_l. admit. *)
-        (* simplify. *)
-        (* unfold hasInputDups. *)
-
-        (* this is annoying (or impossible) to subst... *)
-        (* how did adam deal with the bvector / blist problem? *)
-        (* is this new goal a good place to induct from? (apply more general lemma with calls > i, inductive invariant H1) *)
-        (* whatever postcondition i prove above will become the inductive invariant for calls > i *)
-        admit.
-      }
-      (* i <> 0 *)
-      { assert (i_neq_0 : i <> 0) by omega.
-        apply beq_nat_false_iff in i_neq_0.
-        rewrite i_neq_0.
-        pose proof (beq_nat_refl i) as i_refl.
-        rewrite <- i_refl.
-        clear i_neq_0 i_refl.
-
-        (* replace v_prev with v, since the const vector in front doesn't matter *)
-        eapply comp_spec_eq_trans_r.
-        Focus 2.
-        eapply (compMap_v_eq (forNats blocks) v v_prev).
-        
-        (* should I replace GenUpdate_oc with something else that doesn't use to_list?? *)
-        (* maybe i should replace oracleCompMap inner with hasInputDups (state from Genupdate_oc) first *)
-
-        eapply comp_spec_eq_trans_r.
-        instantiate (1 :=
-                       (a <-$
-      (GenUpdate_oc (k, v) blocks) (list (Blist * Bvector eta))
-        (list_EqDec (pair_EqDec eqdbl (Bvector_EqDec eta))) rb_oracle init;
-                        [_, init'] <-2 a;
-                        ret hasInputDups init')).
-        { fcf_skip_eq.
-          eapply comp_spec_eq_trans_r.
-          destruct b0.
-          simplify.
-          eapply simplify_hasDups.
-          destruct b0.
-          eapply rb_oracle_state_same_after_i.
-          omega.
-        }
-        clear n n0 IHlistLen'.
-        (* TODO apply this same trick to the i=0 case *)
-        apply Gi_rb_collisions_inner_eq.
-      } 
-Qed.
-
-Lemma Gi_rb_bad_eq_2' : forall (i : nat) (v : Bvector eta),
-    Pr [Gi_rb_bad_no_adv i] == Pr[case_on_i i numCalls blocksPerCall v].
-Proof.
-  intros i v.
-
-  fcf_to_prhl_eq.
-  unfold Gi_rb_bad_no_adv.
-  simplify.
-  fcf_irr_l. wfi.
-  simplify.
-  (* clean up left *)
-  eapply comp_spec_eq_trans_r.
-  (* apply simplify_hasDups. *)
-  instantiate (1 :=
-                      (a <-$
-      (oracleCompMap_inner
-         (pair_EqDec (list_EqDec (list_EqDec (Bvector_EqDec eta)))
-            (pair_EqDec nat_EqDec eqDecState))
-         (list_EqDec (list_EqDec (Bvector_EqDec eta))) 
-         (Oi_oc' i) (0%nat, (b, b0)) maxCallsAndBlocks)
-        (list (Blist * Bvector eta))
-        (list_EqDec (pair_EqDec eqdbl (Bvector_EqDec eta))) rb_oracle nil;
-                       [_, state] <-2 a;
-                       ret hasInputDups state)).
-  { prog_equiv. fcf_spec_ret. }
-
-  eapply comp_spec_eq_trans_r.
-  eapply split_out_oracle_call_forall. omega.
-  instantiate (1 := v).
-
-  unfold case_on_i_gen.
-  unfold case_on_i.
-  unfold hasInputDups.
-  Transparent hasDups.
-  simpl. Opaque hasDups.
-  rewrite plus_comm. simpl.
-  destruct (ge_dec i numCalls); destruct (zerop i); try fcf_spec_ret; unfold compMap_v; prog_equiv.
-Qed.
-
 (* probability of bad event happening in RB game is bounded by the probability of collisions in a list of length (n+1) of randomly-sampled (Bvector eta) *)
-
-Require Import RndInList.
-
-Theorem hasDups_cons_orb : 
-  forall (A  : Set)(eqd : EqDec A)(ls : list A)(a : A),
-    hasDups _ (a :: ls) = (if (in_dec (EqDec_dec _) a ls) then true else false) || hasDups _ ls. 
- 
-   intuition.
-   Transparent hasDups.
-   simpl.
-   destruct (in_dec (EqDec_dec eqd) a ls); intuition.
-Qed.
- 
-Theorem compMap_hasDups_cons_orb : 
-  forall (A : Set)(ls : list A) x,
-    Pr[lb <-$ compMap _ (fun _ => {0,1}^eta) ls; ret hasDups _ (x :: lb)] ==
-    Pr[lb <-$ compMap _ (fun _ => {0,1}^eta) ls; ret (if (in_dec (EqDec_dec _) x lb) then true else false) || hasDups _ lb].
-
-  intuition.
-  fcf_skip.
-  rewrite hasDups_cons_orb.
-  intuition.
-
-Qed.
-
-Theorem compMap_hasDups_cons_prob :
-  forall (A : Set)(ls : list A) x, 
-    (Pr[lb <-$ compMap _ (fun _ => {0,1}^eta) ls; ret hasDups _ (x :: lb)] <= S (length ls) ^ 2 / 2 ^ eta)%rat.
-
-  intuition.
-  rewrite compMap_hasDups_cons_orb.
-  rewrite evalDist_orb_le.
-  rewrite FixedInRndList_prob.
-  rewrite dupProb.
-  remember (length ls) as a.
-  rewrite <- ratAdd_den_same.
-  eapply leRat_terms; trivial.
-  simpl.
-  apply le_S.
-  apply plus_le_compat; try omega.
-  apply mult_le_compat; omega.
-Qed.
-
-Close Scope nat.
-Lemma Gi_rb_bad_collisions : forall (i : nat) (v : Bvector eta),
+Lemma Gi_rb_bad_collisions : forall (i : nat),
    Pr  [x <-$ Gi_rb_bad i; ret snd x ] <= Pr_collisions.
 Proof.
   intros.
   rewrite Gi_rb_bad_eq_1.       (* done *)
-  pose proof Gi_rb_bad_eq_2' as select_call.
-  specialize (select_call i v).
-  (* sort of weird to have that v quantified but not mentioned in the theorem statement... *)
-  rewrite select_call. clear select_call.
-  unfold case_on_i.
-  destruct (ge_dec i) as [ i_ge_nc | i_nge_nc ].
-  (* i out of bounds *)
-  - Transparent evalDist. 
-  fcf_compute.
-  apply rat0_le_all.
+  rewrite Gi_rb_bad_eq_2.       (* TODO hard *)
+  rewrite Gi_rb_bad_eq_3.       (* TODO hard *)
+  rewrite Gi_rb_bad_eq_4.       (* done *)
+  rewrite Gi_rb_bad_eq_5.       (* TODO hard / questionable *)
+  rewrite Gi_rb_bad_eq_6.       (* TODO easy *)
+  rewrite Gi_rb_bad_eq_7.       (* TODO easy *)
+  rewrite Gi_rb_bad_eq_8.       (* TODO easy *)
+  unfold Gi_rb_bad_map_inline_v.
+  
+  Opaque hasDups.
+  unfold Pr_collisions.
+  Check dupProb.
+  generalize dupProb.
+  intros dupProb.
 
-  (* i in bounds *)
-  - destruct (zerop i).
-    (* i = 0 *)
-    + 
-     unfold PRG.compMap_v.
-     rewrite compMap_hasDups_cons_prob.
-     rewrite forNats_length.
-     unfold Pr_collisions.
-     eapply leRat_terms; intuition.
-     eapply Nat.pow_le_mono; omega.
-    + 
-    unfold PRG.compMap_v.
-    rewrite compMap_hasDups_cons_prob.
-     rewrite forNats_length.
-     reflexivity.
+(* TODO there's a more general lemma *)
+  assert (length (forNats (S blocksPerCall)) = S blocksPerCall).
+  { apply forNats_length. }
+  rewrite <- H at 2.
+  (* apply Adam's collision bound here *)
+  apply dupProb.
 
+  (* didn't need either of these (work from PRF_DRBG) TODO *)
+  (* apply FixedInRndList_prob. *)
+  (* apply dupProb_const. *)
 Qed.
 
 (* Main theorem (modeled on PRF_DRBG_G3_G4_close) *)
@@ -6435,8 +5414,12 @@ Proof.
 
   (* NOTE still parametrized by i, so the hybrid matters *)
   rewrite Gi_rb_rf_identical_until_bad.
+  (* unfold Gi_rb_bad. unfold PRF_Adversary. simplify. *)
+  (* ??? shouldn't Pr_collisions depend on the hybrid. or just an upper bound? *)
+  (* unfold Pr_collisions. *)
+  (* rb oracle is queried when? i'm confused. only on ith call? yeah only on ith call (when RF is replaced with RB) *)
+  (* so we "zoom in" here and it doesn't really matter if RB before it use new v... or if on the ith call we use new v... only the `bvector eta` getting generated matters? *)
   apply Gi_rb_bad_collisions.
-  bv_exist.
 Qed.
 
 (* for above, want lemmas saying
